src/3d/prelude/EverParse3d.Actions.Base.fsti
@@ -144,6 +144,7 @@ val action
       (on_success:bool)
       (always_succeeds:bool)
       (a:Type0)
+      (use_error_handler:bool)
     : Type0
 
 inline_for_extraction noextract
@@ -158,6 +159,7 @@ val validate_with_action_t
       (l:eloc)
       (has_action:bool)
       (allow_reading:bool)
+      (use_error_handler:bool)
     : Type0
 
 inline_for_extraction noextract
@@ -171,8 +173,9 @@ val validate_eta
       (#[@@@erasable] disj:disjointness_pre)
       (#[@@@erasable] l:eloc)
       (#has_action #allow_reading:bool)
-      (v: validate_with_action_t p inv disj l has_action allow_reading)
-: Tot (validate_with_action_t p inv disj l has_action allow_reading)
+      (#use_error_handler:bool)
+      (v: validate_with_action_t p inv disj l has_action allow_reading use_error_handler)
+: Tot (validate_with_action_t p inv disj l has_action allow_reading use_error_handler)
 
 inline_for_extraction noextract
 val act_with_comment
@@ -181,9 +184,10 @@ val act_with_comment
       (#[@@@erasable] disj:disjointness_pre)
       (#[@@@erasable] l:eloc)
       (#b #rt:_)
+      (#use_error_handler:bool)
       (res:Type)
-      (a: action inv disj l b rt res)
-: Tot (action inv disj l b rt res)
+      (a: action inv disj l b rt res use_error_handler)
+: Tot (action inv disj l b rt res use_error_handler)
 
 inline_for_extraction noextract
 val leaf_reader
@@ -204,8 +208,9 @@ val validate_without_reading
       (#[@@@erasable] disj:disjointness_pre)
       (#[@@@erasable] l:eloc)
       (#has_action #allow_reading:bool)
-      (v: validate_with_action_t p inv disj l has_action allow_reading)
-: Tot (validate_with_action_t p inv disj l has_action false)
+      (#use_error_handler:bool)
+      (v: validate_with_action_t p inv disj l has_action allow_reading use_error_handler)
+: Tot (validate_with_action_t p inv disj l has_action false use_error_handler)
 
 inline_for_extraction noextract
 val validate_with_success_action
@@ -219,13 +224,14 @@ val validate_with_success_action
       (#[@@@erasable] disj1:disjointness_pre)
       (#[@@@erasable] l1:eloc)
       (#has_action #allow_reading:bool)
-      (v1:validate_with_action_t p1 inv1 disj1 l1 has_action allow_reading)
+      (#use_error_handler:bool)
+      (v1:validate_with_action_t p1 inv1 disj1 l1 has_action allow_reading use_error_handler)
       (#[@@@erasable] inv2:slice_inv)
       (#[@@@erasable] disj2:disjointness_pre)
       (#[@@@erasable] l2:eloc)
       (#b #rt:bool)
-      (a:action inv2 disj2 l2 b rt bool)
-  : validate_with_action_t p1 (conj_inv inv1 inv2) (conj_disjointness disj1 disj2) (l1 `eloc_union` l2) true false
+      (a:action inv2 disj2 l2 b rt bool use_error_handler)
+  : validate_with_action_t p1 (conj_inv inv1 inv2) (conj_disjointness disj1 disj2) (l1 `eloc_union` l2) true false use_error_handler
 
 inline_for_extraction noextract
 val validate_with_error_handler
@@ -240,12 +246,14 @@ val validate_with_error_handler
       (#[@@@erasable] disj:disjointness_pre)
       (#[@@@erasable] l1:eloc)
       (#has_action #ar:_)
-      (v1:validate_with_action_t p1 inv1 disj l1 has_action ar)
-  : validate_with_action_t p1 inv1 disj l1 has_action ar
+      (#use_error_handler:bool)
+      (v1:validate_with_action_t p1 inv1 disj l1 has_action ar use_error_handler)
+  : validate_with_action_t p1 inv1 disj l1 has_action ar use_error_handler
 
 inline_for_extraction noextract
 val validate_ret
-  : validate_with_action_t (parse_ret ()) true_inv disjointness_trivial eloc_none false true
+      (#use_error_handler:bool)
+  : validate_with_action_t (parse_ret ()) true_inv disjointness_trivial eloc_none false true use_error_handler
 
 inline_for_extraction noextract
 val validate_pair
@@ -259,7 +267,8 @@ val validate_pair
        (#[@@@erasable] disj1:disjointness_pre)
        (#[@@@erasable] l1:eloc)
        (#has_action1 #allow_reading1:bool)
-       (v1:validate_with_action_t p1 inv1 disj1 l1 has_action1 allow_reading1)
+       (#use_error_handler:bool)
+       (v1:validate_with_action_t p1 inv1 disj1 l1 has_action1 allow_reading1 use_error_handler)
        (#nz2:_)
        (#wk2: _)
        (#k2:parser_kind nz2 wk2)
@@ -270,7 +279,7 @@ val validate_pair
        (#[@@@erasable] disj2:disjointness_pre)
        (#[@@@erasable] l2:eloc)
        (#has_action2 #allow_reading2:bool)
-       (v2:validate_with_action_t p2 inv2 disj2 l2 has_action2 allow_reading2)
+       (v2:validate_with_action_t p2 inv2 disj2 l2 has_action2 allow_reading2 use_error_handler)
   : validate_with_action_t
       (p1 `parse_pair` p2)
       (conj_inv inv1 inv2)
@@ -278,6 +287,7 @@ val validate_pair
       (l1 `eloc_union` l2)
       (has_action1 || has_action2)
       false
+      use_error_handler
 
 inline_for_extraction noextract
 val validate_dep_pair
@@ -290,7 +300,8 @@ val validate_dep_pair
       (#[@@@erasable] disj1:disjointness_pre)
       (#[@@@erasable] l1:eloc)
       (#has_action1:_)
-      (v1:validate_with_action_t p1 inv1 disj1 l1 has_action1 true)
+      (#use_error_handler:bool)
+      (v1:validate_with_action_t p1 inv1 disj1 l1 has_action1 true use_error_handler)
       (r1: leaf_reader p1)
       (#nz2:_)
       (#wk2: _)
@@ -301,7 +312,7 @@ val validate_dep_pair
       (#[@@@erasable] disj2:disjointness_pre)
       (#[@@@erasable] l2:eloc)
       (#has_action2 #allow_reading2:bool)
-      (v2:(x:t1 -> validate_with_action_t (p2 x) inv2 disj2 l2 has_action2 allow_reading2))
+      (v2:(x:t1 -> validate_with_action_t (p2 x) inv2 disj2 l2 has_action2 allow_reading2 use_error_handler))
   : validate_with_action_t
       (p1 `parse_dep_pair` p2)
       (conj_inv inv1 inv2)
@@ -309,6 +320,7 @@ val validate_dep_pair
       (l1 `eloc_union` l2)
       (has_action1 || has_action2)
       false
+      use_error_handler
 
 inline_for_extraction noextract
 val validate_dep_pair_with_refinement_and_action
@@ -322,14 +334,15 @@ val validate_dep_pair_with_refinement_and_action
       (#[@@@erasable] disj1:disjointness_pre)
       (#[@@@erasable] l1:eloc)
       (#has_action1:bool)
-      (v1:validate_with_action_t p1 inv1 disj1 l1 has_action1 true)
+      (#use_error_handler:bool)
+      (v1:validate_with_action_t p1 inv1 disj1 l1 has_action1 true use_error_handler)
       (r1: leaf_reader p1)
       (f: t1 -> bool)
       (#[@@@erasable] inv1':slice_inv)
       (#[@@@erasable] disj1':disjointness_pre)
       (#[@@@erasable] l1':eloc)
       (#b #rt:_)
-      (a:t1 -> action inv1' disj1' l1' b rt bool)
+      (a:t1 -> action inv1' disj1' l1' b rt bool use_error_handler)
       (#nz2:_)
       (#wk2: _)
       (#k2:parser_kind nz2 wk2)
@@ -339,7 +352,7 @@ val validate_dep_pair_with_refinement_and_action
       (#[@@@erasable] disj2:disjointness_pre)
       (#[@@@erasable] l2:eloc)
       (#has_action2 #allow_reading2:bool)
-      (v2:(x:refine _ f -> validate_with_action_t (p2 x) inv2 disj2 l2 has_action2 allow_reading2))
+      (v2:(x:refine _ f -> validate_with_action_t (p2 x) inv2 disj2 l2 has_action2 allow_reading2 use_error_handler))
   : validate_with_action_t
       ((p1 `parse_filter` f) `parse_dep_pair` p2)
       (conj_inv inv1 (conj_inv inv1' inv2))
@@ -347,6 +360,7 @@ val validate_dep_pair_with_refinement_and_action
       (l1 `eloc_union` (l1' `eloc_union` l2))
       true
       false
+      use_error_handler
 
 inline_for_extraction noextract
 val validate_dep_pair_with_action
@@ -358,13 +372,14 @@ val validate_dep_pair_with_action
       (#[@@@erasable] disj1:disjointness_pre)
       (#[@@@erasable] l1:eloc)
       (#has_action1:_)
-      (v1:validate_with_action_t p1 inv1 disj1 l1 has_action1 true)
+      (#use_error_handler:bool)
+      (v1:validate_with_action_t p1 inv1 disj1 l1 has_action1 true use_error_handler)
       (r1: leaf_reader p1)
       (#[@@@erasable] inv1':slice_inv)
       (#[@@@erasable] disj1':disjointness_pre)
       (#[@@@erasable] l1':eloc)
       (#b #rt:_)
-      (a:t1 -> action inv1' disj1' l1' b rt bool)
+      (a:t1 -> action inv1' disj1' l1' b rt bool use_error_handler)
       (#nz2:_)
       (#wk2: _)
       (#k2:parser_kind nz2 wk2)
@@ -374,7 +389,7 @@ val validate_dep_pair_with_action
       (#[@@@erasable] disj2:disjointness_pre)
       (#[@@@erasable] l2:eloc)
       (#has_action2 #allow_reading2:_)
-      (v2:(x:t1 -> validate_with_action_t (p2 x) inv2 disj2 l2 has_action2 allow_reading2))
+      (v2:(x:t1 -> validate_with_action_t (p2 x) inv2 disj2 l2 has_action2 allow_reading2 use_error_handler))
   : validate_with_action_t
       (p1 `(parse_dep_pair #nz1)` p2)
       (conj_inv inv1 (conj_inv inv1' inv2))
@@ -382,6 +397,7 @@ val validate_dep_pair_with_action
       (l1 `eloc_union` (l1' `eloc_union` l2))
       true
       false
+      use_error_handler
 
 inline_for_extraction noextract
 val validate_dep_pair_with_refinement
@@ -395,7 +411,8 @@ val validate_dep_pair_with_refinement
       (#[@@@erasable] disj1:disjointness_pre)      
       (#[@@@erasable] l1:eloc)
       (#has_action1:_)
-      (v1:validate_with_action_t p1 inv1 disj1 l1 has_action1 true)
+      (#use_error_handler:bool)
+      (v1:validate_with_action_t p1 inv1 disj1 l1 has_action1 true use_error_handler)
       (r1: leaf_reader p1)
       (f: t1 -> bool)
       (#nz2:_)
@@ -408,7 +425,7 @@ val validate_dep_pair_with_refinement
       (#[@@@erasable] l2:eloc)
       (#allow_reading2:bool)
       (#has_action2:_)
-      (v2:(x:refine _ f -> validate_with_action_t (p2 x) inv2 disj2 l2 has_action2 allow_reading2))
+      (v2:(x:refine _ f -> validate_with_action_t (p2 x) inv2 disj2 l2 has_action2 allow_reading2 use_error_handler))
   : validate_with_action_t
       ((p1 `parse_filter` f) `parse_dep_pair` p2)
       (conj_inv inv1 inv2)
@@ -416,6 +433,7 @@ val validate_dep_pair_with_refinement
       (l1 `eloc_union` l2)
       (has_action1 || has_action2)
       false
+      use_error_handler
 
 inline_for_extraction noextract
 val validate_filter
@@ -428,12 +446,13 @@ val validate_filter
        (#[@@@erasable] disj:disjointness_pre)                   
        (#[@@@erasable] l:eloc)
        (#has_action:_)
-       (v:validate_with_action_t p inv disj l has_action true)
+       (#use_error_handler:bool)
+       (v:validate_with_action_t p inv disj l has_action true use_error_handler)
        (r:leaf_reader p)
        (f:t -> bool)
        (cr:string)
        (cf:string)
-  : validate_with_action_t (p `parse_filter` f) inv disj l has_action false
+  : validate_with_action_t (p `parse_filter` f) inv disj l has_action false use_error_handler
 
 inline_for_extraction noextract
 val validate_filter_with_action
@@ -446,7 +465,8 @@ val validate_filter_with_action
        (#[@@@erasable] disj:disjointness_pre)                   
        (#[@@@erasable] l:eloc)
        (#has_action:_)
-       (v:validate_with_action_t p inv disj l has_action true)
+       (#use_error_handler:bool)
+       (v:validate_with_action_t p inv disj l has_action true use_error_handler)
        (r:leaf_reader p)
        (f:t -> bool)
        (cr:string)
@@ -455,7 +475,7 @@ val validate_filter_with_action
        (#[@@@erasable] inva:slice_inv)
        (#[@@@erasable] disja:disjointness_pre)                   
        (#[@@@erasable] la:eloc)
-       (a: t -> action inva disja la b rt bool)
+       (a: t -> action inva disja la b rt bool use_error_handler)
   : validate_with_action_t #nz
       (p `parse_filter` f)
       (conj_inv inv inva)
@@ -463,6 +483,7 @@ val validate_filter_with_action
       (eloc_union l la)
       true
       false
+      use_error_handler
 
 inline_for_extraction noextract
 val validate_with_dep_action
@@ -475,13 +496,14 @@ val validate_with_dep_action
        (#[@@@erasable] disj:disjointness_pre)                   
        (#[@@@erasable] l:eloc)
        (#has_action:_)
-       (v:validate_with_action_t p inv disj l has_action true)
+       (#use_error_handler:bool)
+       (v:validate_with_action_t p inv disj l has_action true use_error_handler)
        (r:leaf_reader p)
        (#b #rt:bool)
        (#[@@@erasable] inva:slice_inv)
        (#[@@@erasable] disja:disjointness_pre)                   
        (#[@@@erasable] la:eloc)
-       (a: t -> action inva disja la b rt bool)
+       (a: t -> action inva disja la b rt bool use_error_handler)
   : validate_with_action_t #nz
       p
       (conj_inv inv inva)
@@ -489,6 +511,7 @@ val validate_with_dep_action
       (eloc_union l la)
       true
       false
+      use_error_handler
 
 inline_for_extraction noextract
 val validate_weaken_left
@@ -502,11 +525,12 @@ val validate_weaken_left
        (#[@@@erasable] l:eloc)
        (#allow_reading:bool)
        (#has_action:_)
-       (v:validate_with_action_t p inv disj l has_action allow_reading)
+       (#use_error_handler:bool)
+       (v:validate_with_action_t p inv disj l has_action allow_reading use_error_handler)
        (#nz':_)
        (#wk': _)
        (k':parser_kind nz' wk')
-  : validate_with_action_t (parse_weaken_left p k') inv disj l has_action allow_reading
+  : validate_with_action_t (parse_weaken_left p k') inv disj l has_action allow_reading use_error_handler
 
 inline_for_extraction noextract
 val validate_weaken_right
@@ -520,16 +544,18 @@ val validate_weaken_right
        (#[@@@erasable] l:eloc)
        (#allow_reading:bool)
        (#has_action:_)
-       (v:validate_with_action_t p inv disj l has_action allow_reading)
+       (#use_error_handler:bool)
+       (v:validate_with_action_t p inv disj l has_action allow_reading use_error_handler)
        (#nz':_)
        (#wk': _)
        (k':parser_kind nz' wk')
-  : validate_with_action_t (parse_weaken_right p k') inv disj l has_action allow_reading
+  : validate_with_action_t (parse_weaken_right p k') inv disj l has_action allow_reading use_error_handler
 
 inline_for_extraction noextract
 val validate_impos
+       (#use_error_handler:bool)
        (_:unit)
-  : validate_with_action_t (parse_impos ()) true_inv disjointness_trivial eloc_none false true
+  : validate_with_action_t (parse_impos ()) true_inv disjointness_trivial eloc_none false true use_error_handler
 
 noextract inline_for_extraction
 val validate_ite
@@ -547,10 +573,11 @@ val validate_ite
        (#[@@@erasable] disj2:disjointness_pre)
        (#[@@@erasable] l2:eloc)
        (#ha2 #ar2:_)
+       (#use_error_handler:bool)
        ([@@@erasable] p1:squash e -> parser k (a()))
-       (v1:(squash e -> validate_with_action_t (p1()) inv1 disj1 l1 ha1 ar1))
+       (v1:(squash e -> validate_with_action_t (p1()) inv1 disj1 l1 ha1 ar1 use_error_handler))
        ([@@@erasable] p2:squash (not e) -> parser k (b()))
-       (v2:(squash (not e) -> validate_with_action_t (p2()) inv2 disj2 l2 ha2 ar2))
+       (v2:(squash (not e) -> validate_with_action_t (p2()) inv2 disj2 l2 ha2 ar2 use_error_handler))
   : validate_with_action_t
       (parse_ite e p1 p2)
       (conj_inv inv1 inv2)
@@ -558,6 +585,7 @@ val validate_ite
       (l1 `eloc_union` l2)
       (ha1 || ha2)
       false
+      use_error_handler
 
 noextract inline_for_extraction
 val validate_nlist
@@ -571,8 +599,9 @@ val validate_nlist
        (#[@@@erasable] disj:disjointness_pre)                   
        (#[@@@erasable] l:eloc)
        (#ha #allow_reading:bool)
-       (v: validate_with_action_t p inv disj l ha allow_reading)
-: validate_with_action_t (parse_nlist n n_is_const p) inv disj l ha false
+       (#use_error_handler:bool)
+       (v: validate_with_action_t p inv disj l ha allow_reading use_error_handler)
+: validate_with_action_t (parse_nlist n n_is_const p) inv disj l ha false use_error_handler
 
 noextract inline_for_extraction
 val validate_nlist_constant_size_without_actions
@@ -587,8 +616,9 @@ val validate_nlist_constant_size_without_actions
        (#[@@@erasable] disj:disjointness_pre)                   
        (#[@@@erasable] l:eloc)
        (#allow_reading:bool)
-       (v: validate_with_action_t p inv disj l false allow_reading)
-: Tot (validate_with_action_t (parse_nlist n n_is_const p) inv disj l false false)
+       (#use_error_handler:bool)
+       (v: validate_with_action_t p inv disj l false allow_reading use_error_handler)
+: Tot (validate_with_action_t (parse_nlist n n_is_const p) inv disj l false false use_error_handler)
 
 noextract inline_for_extraction
 val validate_t_at_most
@@ -602,8 +632,9 @@ val validate_t_at_most
        (#[@@@erasable] disj:disjointness_pre)                   
        (#[@@@erasable] l:eloc)
        (#ha #ar:_)
-       (v:validate_with_action_t p inv disj l ha ar)
-  : Tot (validate_with_action_t (parse_t_at_most n p) inv disj l ha false)
+       (#use_error_handler:bool)
+       (v:validate_with_action_t p inv disj l ha ar use_error_handler)
+  : Tot (validate_with_action_t (parse_t_at_most n p) inv disj l ha false use_error_handler)
 
 noextract inline_for_extraction
 val validate_t_exact
@@ -617,8 +648,9 @@ val validate_t_exact
        (#[@@@erasable] disj:disjointness_pre)                   
        (#[@@@erasable] l:eloc)
        (#ha #ar:_)
-       (v:validate_with_action_t p inv disj l ha ar)
-  : Tot (validate_with_action_t (parse_t_exact n p) inv disj l ha false)
+       (#use_error_handler:bool)
+       (v:validate_with_action_t p inv disj l ha ar use_error_handler)
+  : Tot (validate_with_action_t (parse_t_exact n p) inv disj l ha false use_error_handler)
 
 inline_for_extraction noextract
 val validate_with_comment
@@ -632,8 +664,9 @@ val validate_with_comment
        (#[@@@erasable] disj:disjointness_pre)                   
        (#[@@@erasable] l:eloc)
        (#ha #allow_reading:bool)
-       (v:validate_with_action_t p inv disj l ha allow_reading)
-  : validate_with_action_t p inv disj l ha allow_reading
+       (#use_error_handler:bool)
+       (v:validate_with_action_t p inv disj l ha allow_reading use_error_handler)
+  : validate_with_action_t p inv disj l ha allow_reading use_error_handler
 
 inline_for_extraction noextract
 val validate_weaken_inv_loc
@@ -646,11 +679,12 @@ val validate_weaken_inv_loc
        (#[@@@erasable] disj:disjointness_pre)                   
        (#[@@@erasable] l:eloc)
        (#ha #allow_reading:bool)
+       (#use_error_handler:bool)
        ([@@@erasable] inv':slice_inv{inv' `inv_implies` inv})
        ([@@@erasable] disj':disjointness_pre { disj' `imp_disjointness` disj })
        ([@@@erasable] l':eloc{l' `eloc_includes` l})
-       (v:validate_with_action_t p inv disj l ha allow_reading)
-  : Tot (validate_with_action_t p inv' disj' l' ha allow_reading)
+       (v:validate_with_action_t p inv disj l ha allow_reading use_error_handler)
+  : Tot (validate_with_action_t p inv' disj' l' ha allow_reading use_error_handler)
 
 inline_for_extraction noextract
 val read_filter
@@ -667,88 +701,88 @@ val read_impos
     : leaf_reader (parse_impos())
 
 inline_for_extraction
-let validator #nz #wk (#k:parser_kind nz wk) (#t:Type) (p:parser k t)
-  = validate_with_action_t p true_inv disjointness_trivial eloc_none false true
+let validator #nz #wk (#k:parser_kind nz wk) (#t:Type) (p:parser k t) (#use_error_handler:bool)
+  = validate_with_action_t p true_inv disjointness_trivial eloc_none false true use_error_handler
 
 inline_for_extraction
-let validator_maybe_action #nz #wk (#k:parser_kind nz wk) (#t:Type) (p:parser k t) (has_action:bool)
-  = validate_with_action_t p true_inv disjointness_trivial eloc_none has_action true
+let validator_maybe_action #nz #wk (#k:parser_kind nz wk) (#t:Type) (p:parser k t) (has_action:bool) (#use_error_handler:bool)
+  = validate_with_action_t p true_inv disjointness_trivial eloc_none has_action true use_error_handler
 
 inline_for_extraction noextract
-val validate____UINT8
-  : validator parse____UINT8
+val validate____UINT8 (#use_error_handler:bool)
+  : validator parse____UINT8 #use_error_handler
 
 inline_for_extraction noextract
 val read____UINT8
   : leaf_reader parse____UINT8
 
 inline_for_extraction noextract
-val validate____UINT8BE
-  : validator parse____UINT8BE
+val validate____UINT8BE (#use_error_handler:bool)
+  : validator parse____UINT8BE #use_error_handler
 
 inline_for_extraction noextract
 val read____UINT8BE
   : leaf_reader parse____UINT8BE
 
 inline_for_extraction noextract
-val validate____UINT16BE
-  : validator parse____UINT16BE
+val validate____UINT16BE (#use_error_handler:bool)
+  : validator parse____UINT16BE #use_error_handler
 
 inline_for_extraction noextract
 val read____UINT16BE
   : leaf_reader parse____UINT16BE
 
 inline_for_extraction noextract
-val validate____UINT32BE
-  : validator parse____UINT32BE
+val validate____UINT32BE (#use_error_handler:bool)
+  : validator parse____UINT32BE #use_error_handler
 
 inline_for_extraction noextract
 val read____UINT32BE
   : leaf_reader parse____UINT32BE
 
 inline_for_extraction noextract
-val validate____UINT64BE
-  : validator parse____UINT64BE
+val validate____UINT64BE (#use_error_handler:bool)
+  : validator parse____UINT64BE #use_error_handler
 
 inline_for_extraction noextract
 val read____UINT64BE
   : leaf_reader parse____UINT64BE
 
 inline_for_extraction noextract
-val validate____UINT16
-  : validator parse____UINT16
+val validate____UINT16 (#use_error_handler:bool)
+  : validator parse____UINT16 #use_error_handler
 
 inline_for_extraction noextract
 val read____UINT16
   : leaf_reader parse____UINT16
 
 inline_for_extraction noextract
-val validate____UINT32
-  : validator parse____UINT32
+val validate____UINT32 (#use_error_handler:bool)
+  : validator parse____UINT32 #use_error_handler
 
 inline_for_extraction noextract
 val read____UINT32
   : leaf_reader parse____UINT32
 
 inline_for_extraction noextract
-val validate____UINT64
-  : validator parse____UINT64
+val validate____UINT64 (#use_error_handler:bool)
+  : validator parse____UINT64 #use_error_handler
 
 inline_for_extraction noextract
 val read____UINT64
   : leaf_reader parse____UINT64
 
 inline_for_extraction noextract
-val validate_unit
-  : validator parse_unit
+val validate_unit (#use_error_handler:bool)
+  : validator parse_unit #use_error_handler
 
 inline_for_extraction noextract
 val read_unit
   : leaf_reader (parse_ret ())
 
 inline_for_extraction noextract
-val validate_unit_refinement (f:unit -> bool) (cf:string)
-  : validator (parse_unit `parse_filter` f)
+val validate_unit_refinement (f:unit -> bool) (cf:string) (#use_error_handler:bool)
+  : validator (parse_unit `parse_filter` f) #use_error_handler
 
 inline_for_extraction noextract
 val validate_string
@@ -756,18 +790,19 @@ val validate_string
        (#t: eqtype)
        (#[@@@erasable] p: parser k t)
        (#ha:_)
-       (v: validator_maybe_action p ha)
+       (#use_error_handler:bool)
+       (v: validator_maybe_action p ha #use_error_handler)
        (r: leaf_reader p)
        (terminator: t)
-  : Tot (validate_with_action_t (parse_string p terminator) true_inv disjointness_trivial eloc_none ha false)
+  : Tot (validate_with_action_t (parse_string p terminator) true_inv disjointness_trivial eloc_none ha false use_error_handler)
 
 inline_for_extraction noextract
-val validate_all_bytes
-  : validate_with_action_t parse_all_bytes true_inv disjointness_trivial eloc_none false false // could be true
+val validate_all_bytes (#use_error_handler:bool)
+  : validate_with_action_t parse_all_bytes true_inv disjointness_trivial eloc_none false false use_error_handler // could be true
 
 inline_for_extraction noextract
-val validate_all_zeros
-  : validate_with_action_t parse_all_zeros true_inv disjointness_trivial eloc_none false false
+val validate_all_zeros (#use_error_handler:bool)
+  : validate_with_action_t parse_all_zeros true_inv disjointness_trivial eloc_none false false use_error_handler
 
 ////////////////////////////////////////////////////////////////////////////////
 
@@ -776,12 +811,13 @@ inline_for_extraction
 val action_return
       (#a:Type)
       (x:a)
-  : action true_inv disjointness_trivial eloc_none false false a
+      (#use_error_handler:bool)
+  : action true_inv disjointness_trivial eloc_none false false a use_error_handler
 
 noextract
 inline_for_extraction
-val action_return_true
-  : action true_inv disjointness_trivial eloc_none false true bool
+val action_return_true (#use_error_handler:bool)
+  : action true_inv disjointness_trivial eloc_none false true bool use_error_handler
 
 noextract
 inline_for_extraction
@@ -792,13 +828,14 @@ val action_bind
       (#[@@@erasable] lf:eloc)
       (#bf #rtf:_)
       (#a:Type)
-      (f: action invf disjf lf bf rtf a)
+      (#use_error_handler:bool)
+      (f: action invf disjf lf bf rtf a use_error_handler)
       (#[@@@erasable] invg:slice_inv)
       (#[@@@erasable] disjg:disjointness_pre)
       (#[@@@erasable] lg:eloc)
       (#bg #rt:_)
       (#b:Type)
-      (g: (a -> action invg disjg lg bg rt b))
+      (g: (a -> action invg disjg lg bg rt b use_error_handler))
   : action
       (conj_inv invf invg)
       (conj_disjointness disjf disjg)
@@ -806,6 +843,7 @@ val action_bind
       (bf || bg)
       rt
       b
+      use_error_handler
 
 noextract
 inline_for_extraction
@@ -815,13 +853,14 @@ val action_seq
       (#[@@@erasable] lf:eloc)
       (#bf #rtf:_)
       (#a:Type)
-      (f: action invf disjf lf bf rtf a)
+      (#use_error_handler:bool)
+      (f: action invf disjf lf bf rtf a use_error_handler)
       (#[@@@erasable] invg:slice_inv)
       (#[@@@erasable] disjg:disjointness_pre)
       (#[@@@erasable] lg:eloc)
       (#bg #rtg:_)
       (#b:Type)
-      (g: action invg disjg lg bg rtg b)
+      (g: action invg disjg lg bg rtg b use_error_handler)
   : action
       (conj_inv invf invg)
       (conj_disjointness disjf disjg)
@@ -829,6 +868,7 @@ val action_seq
       (bf || bg)
       rtg
       b
+      use_error_handler
 
 noextract
 inline_for_extraction
@@ -839,12 +879,13 @@ val action_ite
       (guard:bool)
       (#bf #rtf:_)
       (#a:Type)
-      (then_: squash guard -> action invf disjf lf bf rtf a)
+      (#use_error_handler:bool)
+      (then_: squash guard -> action invf disjf lf bf rtf a use_error_handler)
       (#[@@@erasable] invg:slice_inv)
       (#[@@@erasable] disjg:disjointness_pre)
       (#[@@@erasable] lg:eloc)
       (#bg #rtg:_)
-      (else_: squash (not guard) -> action invg disjg lg bg rtg a)
+      (else_: squash (not guard) -> action invg disjg lg bg rtg a use_error_handler)
   : action
       (conj_inv invf invg)
       (conj_disjointness disjf disjg)
@@ -852,23 +893,25 @@ val action_ite
       (bf || bg)
       (rtf && rtg)
       a
+      use_error_handler
 
 noextract
 inline_for_extraction
-val action_abort      
-  : action true_inv disjointness_trivial eloc_none false false bool
+val action_abort (#use_error_handler:bool)
+  : action true_inv disjointness_trivial eloc_none false false bool use_error_handler
 
 noextract
 inline_for_extraction
-val action_field_pos_64
-   : action true_inv disjointness_trivial eloc_none false false U64.t
+val action_field_pos_64 (#use_error_handler:bool)
+   : action true_inv disjointness_trivial eloc_none false false U64.t use_error_handler
 
 noextract
 inline_for_extraction
 val action_deref
       (#a:_)
       (x:bpointer a)
-   : action (ptr_inv x) disjointness_trivial eloc_none false false a
+      (#use_error_handler:bool)
+   : action (ptr_inv x) disjointness_trivial eloc_none false false a use_error_handler
 
 noextract
 inline_for_extraction
@@ -876,7 +919,8 @@ val action_assignment
       (#a:_)
       (x:bpointer a)
       (v:a)
-   : action (ptr_inv x) disjointness_trivial (ptr_loc x) false false unit
+      (#use_error_handler:bool)
+   : action (ptr_inv x) disjointness_trivial (ptr_loc x) false false unit use_error_handler
 
 noextract
 inline_for_extraction
@@ -886,11 +930,12 @@ val action_weaken
       (#[@@@erasable] l:eloc)
       (#b #rt:_)
       (#a:_)
-      (act:action inv disj l b rt a)
+      (#use_error_handler:bool)
+      (act:action inv disj l b rt a use_error_handler)
       (#[@@@erasable] inv':slice_inv{inv' `inv_implies` inv})
       (#[@@@erasable] disj':disjointness_pre { disj' `imp_disjointness` disj })
       (#l':eloc{l' `eloc_includes` l})
-   : action inv' disj' l' b rt a
+   : action inv' disj' l' b rt a use_error_handler
 
 inline_for_extraction
 noextract
@@ -901,7 +946,8 @@ inline_for_extraction
 val mk_external_action
   (#t: Type)
   (#l:eloc) ($f: external_action t l)
-  : action true_inv disjointness_trivial l false false t
+  (#use_error_handler:bool)
+  : action true_inv disjointness_trivial l false false t use_error_handler
 
 val copy_buffer_inv (x:CP.copy_buffer_t) : slice_inv
 val copy_buffer_loc (x:CP.copy_buffer_t) : eloc
@@ -921,9 +967,10 @@ val probe_then_validate
       (#l:eloc)
       (#ha #allow_reading:bool)
       (#ptr_t:Type0)
+      (#use_error_handler:bool)
       (typename:string)
       (fieldname:string)
-      (v:validate_with_action_t p inv disj l ha allow_reading)
+      (v:validate_with_action_t p inv disj l ha allow_reading use_error_handler)
       (src:ptr_t)
       (as_u64: ptr_t -> PA.pure_external_action U64.t)
       (nullable:bool)
@@ -937,6 +984,7 @@ val probe_then_validate
            true
            false
            bool
+           use_error_handler
 
 // Some actions are valid only for specific backends (buffer, extern, etc.)
 
