src/3d/Options.fst
@@ -135,6 +135,8 @@ let z3_options : ref (option vstring) = alloc None
 
 let z3_skip_c_initializers: ref bool = alloc false
 
+let use_error_handler_macro : ref bool = alloc false
+
 let char_le (c1 c2: FStar.Char.char) : Tot bool =
   FStar.Char.int_of_char c1 <= FStar.Char.int_of_char c2
 
@@ -400,6 +402,7 @@ let (display_usage_2, compute_options_2, fstar_options) =
     CmdOption "z3_options" (OptStringOption "'options to z3'" always_valid z3_options) "command-line options to pass to z3 for test case generation (does not affect verification of generated F* code)" [];
     CmdOption "z3_skip_testcases_c" (OptBool no_produce_testcases_c) "skip generating test cases to <output directory>/testcases.c" [];
     CmdOption "z3_skip_c_initializers" (OptBool z3_skip_c_initializers) "Do not use C field initializers for test cases" [];
+    CmdOption "use_error_handler_macro" (OptBool use_error_handler_macro) "Use the C macro `EverParse3dErrorHandlerMacro` instead of the dynamic error handler" [];
     CmdOption "z3_test" (OptStringOption "parser name" always_valid z3_test) "produce positive and/or negative test cases for a given parser" [];
     CmdOption "z3_test_mode" (OptStringOption "pos|neg|all" valid_z3_test_mode z3_test_mode) "produce positive, negative, or all kinds of test cases (default all)" [];
     CmdOption "z3_use_ptr" (OptBool use_ptr_for_probe) "use pointers rather than array indices for probes" [];
@@ -661,6 +664,9 @@ let get_produce_testcases_c () : ML bool =
 
 let get_z3_skip_c_initializers () : ML bool =
   !z3_skip_c_initializers
+
+let get_use_error_handler_macro () : ML bool =
+  !use_error_handler_macro
 
 let get_z3_use_ptr () : ML bool =
   !use_ptr_for_probe
